coq/ExecutionTreeOpt.v
@@ -13,7 +13,6 @@ From SE Require Import LLVMAst.
 From SE Require Import ModuleAssumptions.
 From SE Require Import Symbolic.
 From SE Require Import Relation.
-From SE Require Import WellDefinedness.
 
 From SE.SMT Require Import Expr.
 From SE.SMT Require Import Model.
